EvmEquivalence/Equivalence/SloadEquivalence.lean
@@ -1,0 +1,711 @@
+import EvmEquivalence.Summaries.SloadSummary
+import EvmEquivalence.Interfaces.EvmYulInterface
+import EvmEquivalence.Interfaces.GasInterface
+import EvmEquivalence.Interfaces.FuncInterface
+import EvmEquivalence.StateMap
+
+open EvmYul
+open StateMap
+open KEVMInterface
+open SloadSummary
+
+namespace SloadOpcodeEquivalence
+
+def sloadLHS
+  {ACCESSEDSTORAGE_CELL : SortMap}
+  {GAS_CELL ID_CELL PC_CELL W0 : SortInt}
+  {K_CELL : SortK}
+  {SCHEDULE_CELL : SortSchedule}
+  {USEGAS_CELL : SortBool}
+  {WS : SortWordStack}
+  {_DotVar0 : SortGeneratedCounterCell}
+  {_DotVar6 _Val9 : SortAccountCellMap}
+  {_Gen0 : SortProgramCell}
+  {_Gen1 : SortJumpDestsCell}
+  {_Gen10 : SortSelfDestructCell}
+  {_Gen11 : SortLogCell}
+  {_Gen12 : SortRefundCell}
+  {_Gen13 : SortAccessedAccountsCell}
+  {_Gen14 : SortCreatedAccountsCell}
+  {_Gen15 : SortOutputCell}
+  {_Gen16 : SortStatusCodeCell}
+  {_Gen17 : SortCallStackCell}
+  {_Gen18 : SortInterimStatesCell}
+  {_Gen19 : SortTouchedAccountsCell}
+  {_Gen2 : SortCallerCell}
+  {_Gen20 : SortVersionedHashesCell}
+  {_Gen21 : SortGasPriceCell}
+  {_Gen22 : SortOriginCell}
+  {_Gen23 : SortBlockhashesCell}
+  {_Gen24 : SortBlockCell}
+  {_Gen25 : SortBalanceCell}
+  {_Gen26 : SortCodeCell}
+  {_Gen27 : SortOrigStorageCell}
+  {_Gen28 : SortTransientStorageCell}
+  {_Gen29 : SortNonceCell}
+  {_Gen3 : SortCallDataCell}
+  {_Gen30 : SortChainIDCell}
+  {_Gen31 : SortTxOrderCell}
+  {_Gen32 : SortTxPendingCell}
+  {_Gen33 : SortMessagesCell}
+  {_Gen34 : SortWithdrawalsPendingCell}
+  {_Gen35 : SortWithdrawalsOrderCell}
+  {_Gen36 : SortWithdrawalsCell}
+  {_Gen37 : SortExitCodeCell}
+  {_Gen38 : SortModeCell}
+  {_Gen4 : SortCallValueCell}
+  {_Gen5 : SortLocalMemCell}
+  {_Gen6 : SortMemoryUsedCell}
+  {_Gen7 : SortCallGasCell}
+  {_Gen8 : SortStaticCell}
+  {_Gen9 : SortCallDepthCell} : SortGeneratedTopCell :=
+  {kevm := {
+        k := { val := SortK.kseq ((@inj SortInternalOp SortKItem) (SortInternalOp.«#next[_]_EVM_InternalOp_MaybeOpCode» ((@inj SortUnStackOp SortMaybeOpCode) SortUnStackOp.SLOAD_EVM_UnStackOp))) K_CELL },
+        exitCode := _Gen37,
+        mode := _Gen38,
+        schedule := { val := SCHEDULE_CELL },
+        useGas := { val := USEGAS_CELL },
+        ethereum := {
+          evm := {
+            output := _Gen15,
+            statusCode := _Gen16,
+            callStack := _Gen17,
+            interimStates := _Gen18,
+            touchedAccounts := _Gen19,
+            callState := {
+              program := _Gen0,
+              jumpDests := _Gen1,
+              id := { val := (@inj SortInt SortAccount) ID_CELL },
+              caller := _Gen2,
+              callData := _Gen3,
+              callValue := _Gen4,
+              wordStack := { val := SortWordStack.«_:__EVM-TYPES_WordStack_Int_WordStack» W0 WS },
+              localMem := _Gen5,
+              pc := { val := PC_CELL },
+              gas := { val := (@inj SortInt SortGas) GAS_CELL },
+              memoryUsed := _Gen6,
+              callGas := _Gen7,
+              static := _Gen8,
+              callDepth := _Gen9 },
+            versionedHashes := _Gen20,
+            substate := {
+              selfDestruct := _Gen10,
+              log := _Gen11,
+              refund := _Gen12,
+              accessedAccounts := _Gen13,
+              accessedStorage := { val := ACCESSEDSTORAGE_CELL },
+              createdAccounts := _Gen14 },
+            gasPrice := _Gen21,
+            origin := _Gen22,
+            blockhashes := _Gen23,
+            block := _Gen24 },
+          network := {
+            chainID := _Gen30,
+            accounts := { val := _Val9 },
+            txOrder := _Gen31,
+            txPending := _Gen32,
+            messages := _Gen33,
+            withdrawalsPending := _Gen34,
+            withdrawalsOrder := _Gen35,
+            withdrawals := _Gen36 } } },
+      generatedCounter := _DotVar0 }
+
+def sloadRHS
+  {_Val22 : SortMap}
+  {ID_CELL _Val10 _Val11 _Val13 _Val14 _Val15 _Val16 _Val2 _Val3 _Val4 : SortInt}
+  {K_CELL : SortK}
+  {SCHEDULE_CELL : SortSchedule}
+  {_Val0 _Val1 _Val12 _Val5 _Val6 _Val7 : SortBool}
+  {WS : SortWordStack}
+  {_DotVar0 : SortGeneratedCounterCell}
+  {_DotVar6 _Val23 _Val24 _Val8 _Val9 : SortAccountCellMap}
+  {_Gen0 : SortProgramCell}
+  {_Gen1 : SortJumpDestsCell}
+  {_Gen10 : SortSelfDestructCell}
+  {_Gen11 : SortLogCell}
+  {_Gen12 : SortRefundCell}
+  {_Gen13 : SortAccessedAccountsCell}
+  {_Gen14 : SortCreatedAccountsCell}
+  {_Gen15 : SortOutputCell}
+  {_Gen16 : SortStatusCodeCell}
+  {_Gen17 : SortCallStackCell}
+  {_Gen18 : SortInterimStatesCell}
+  {_Gen19 : SortTouchedAccountsCell}
+  {_Gen2 : SortCallerCell}
+  {_Gen20 : SortVersionedHashesCell}
+  {_Gen21 : SortGasPriceCell}
+  {_Gen22 : SortOriginCell}
+  {_Gen23 : SortBlockhashesCell}
+  {_Gen24 : SortBlockCell}
+  {_Gen25 : SortBalanceCell}
+  {_Gen26 : SortCodeCell}
+  {_Gen27 : SortOrigStorageCell}
+  {_Gen28 : SortTransientStorageCell}
+  {_Gen29 : SortNonceCell}
+  {_Gen3 : SortCallDataCell}
+  {_Gen30 : SortChainIDCell}
+  {_Gen31 : SortTxOrderCell}
+  {_Gen32 : SortTxPendingCell}
+  {_Gen33 : SortMessagesCell}
+  {_Gen34 : SortWithdrawalsPendingCell}
+  {_Gen35 : SortWithdrawalsOrderCell}
+  {_Gen36 : SortWithdrawalsCell}
+  {_Gen37 : SortExitCodeCell}
+  {_Gen38 : SortModeCell}
+  {_Gen4 : SortCallValueCell}
+  {_Gen5 : SortLocalMemCell}
+  {_Gen6 : SortMemoryUsedCell}
+  {_Gen7 : SortCallGasCell}
+  {_Gen8 : SortStaticCell}
+  {_Gen9 : SortCallDepthCell}
+  {_Val17 _Val19 _Val20 _Val21 : SortSet}
+  {_Val18 : SortKItem} : SortGeneratedTopCell :=
+  { kevm := {
+      k := { val := K_CELL },
+      exitCode := _Gen37,
+      mode := _Gen38,
+      schedule := { val := SCHEDULE_CELL },
+      useGas := { val := true },
+      ethereum := {
+        evm := {
+          output := _Gen15,
+          statusCode := _Gen16,
+          callStack := _Gen17,
+          interimStates := _Gen18,
+          touchedAccounts := _Gen19,
+          callState := {
+            program := _Gen0,
+            jumpDests := _Gen1,
+            id := { val := (@inj SortInt SortAccount) ID_CELL },
+            caller := _Gen2,
+            callData := _Gen3,
+            callValue := _Gen4,
+            wordStack := { val := SortWordStack.«_:__EVM-TYPES_WordStack_Int_WordStack» _Val10 WS },
+            localMem := _Gen5,
+            pc := { val := _Val11 },
+            gas := { val := (@inj SortInt SortGas) _Val16 },
+            memoryUsed := _Gen6,
+            callGas := _Gen7,
+            static := _Gen8,
+            callDepth := _Gen9 },
+          versionedHashes := _Gen20,
+          substate := {
+            selfDestruct := _Gen10,
+            log := _Gen11,
+            refund := _Gen12,
+            accessedAccounts := _Gen13,
+            accessedStorage := { val := _Val22 },
+            createdAccounts := _Gen14 },
+          gasPrice := _Gen21,
+          origin := _Gen22,
+          blockhashes := _Gen23,
+          block := _Gen24 },
+        network := {
+          chainID := _Gen30,
+          accounts := { val := _Val24 },
+          txOrder := _Gen31,
+          txPending := _Gen32,
+          messages := _Gen33,
+          withdrawalsPending := _Gen34,
+          withdrawalsOrder := _Gen35,
+          withdrawals := _Gen36 } } },
+      generatedCounter := _DotVar0 }
+
+theorem rw_sloadLHS_sloadRHS
+  {ACCESSEDSTORAGE_CELL STORAGE_CELL _Val22 : SortMap}
+  {GAS_CELL ID_CELL PC_CELL W0 _Val10 _Val11 _Val13 _Val14 _Val15 _Val16 _Val2 _Val3 _Val4 : SortInt}
+  {K_CELL : SortK}
+  {SCHEDULE_CELL : SortSchedule}
+  {USEGAS_CELL _Val0 _Val1 _Val12 _Val5 _Val6 _Val7 : SortBool}
+  {WS : SortWordStack}
+  {_DotVar0 : SortGeneratedCounterCell}
+  {_DotVar6 _Val23 _Val24 _Val8 _Val9 : SortAccountCellMap}
+  {_Gen0 : SortProgramCell}
+  {_Gen1 : SortJumpDestsCell}
+  {_Gen10 : SortSelfDestructCell}
+  {_Gen11 : SortLogCell}
+  {_Gen12 : SortRefundCell}
+  {_Gen13 : SortAccessedAccountsCell}
+  {_Gen14 : SortCreatedAccountsCell}
+  {_Gen15 : SortOutputCell}
+  {_Gen16 : SortStatusCodeCell}
+  {_Gen17 : SortCallStackCell}
+  {_Gen18 : SortInterimStatesCell}
+  {_Gen19 : SortTouchedAccountsCell}
+  {_Gen2 : SortCallerCell}
+  {_Gen20 : SortVersionedHashesCell}
+  {_Gen21 : SortGasPriceCell}
+  {_Gen22 : SortOriginCell}
+  {_Gen23 : SortBlockhashesCell}
+  {_Gen24 : SortBlockCell}
+  {_Gen25 : SortBalanceCell}
+  {_Gen26 : SortCodeCell}
+  {_Gen27 : SortOrigStorageCell}
+  {_Gen28 : SortTransientStorageCell}
+  {_Gen29 : SortNonceCell}
+  {_Gen3 : SortCallDataCell}
+  {_Gen30 : SortChainIDCell}
+  {_Gen31 : SortTxOrderCell}
+  {_Gen32 : SortTxPendingCell}
+  {_Gen33 : SortMessagesCell}
+  {_Gen34 : SortWithdrawalsPendingCell}
+  {_Gen35 : SortWithdrawalsOrderCell}
+  {_Gen36 : SortWithdrawalsCell}
+  {_Gen37 : SortExitCodeCell}
+  {_Gen38 : SortModeCell}
+  {_Gen4 : SortCallValueCell}
+  {_Gen5 : SortLocalMemCell}
+  {_Gen6 : SortMemoryUsedCell}
+  {_Gen7 : SortCallGasCell}
+  {_Gen8 : SortStaticCell}
+  {_Gen9 : SortCallDepthCell}
+  {_Val17 _Val19 _Val20 _Val21 : SortSet}
+  {_Val18 : SortKItem}
+  (defn_Val0 : «_<<_>>_SCHEDULE_Bool_ScheduleFlag_Schedule» SortScheduleFlag.Ghasaccesslist_SCHEDULE_ScheduleFlag SCHEDULE_CELL = some _Val0)
+  (defn_Val1 : «#inStorage» ACCESSEDSTORAGE_CELL ((@inj SortInt SortAccount) ID_CELL) W0 = some _Val1)
+  (defn_Val2 : «_<_>_SCHEDULE_Int_ScheduleConst_Schedule» SortScheduleConst.Gwarmstorageread_SCHEDULE_ScheduleConst SCHEDULE_CELL = some _Val2)
+  (defn_Val3 : «_<_>_SCHEDULE_Int_ScheduleConst_Schedule» SortScheduleConst.Gcoldsload_SCHEDULE_ScheduleConst SCHEDULE_CELL = some _Val3)
+  (defn_Val4 : kite _Val1 _Val2 _Val3 = some _Val4)
+  (defn_Val5 : «_<=Int_» _Val4 GAS_CELL = some _Val5)
+  (defn_Val6 : _andBool_ _Val0 _Val5 = some _Val6)
+  (defn_Val7 : _andBool_ USEGAS_CELL _Val6 = some _Val7)
+  (defn_Val8 : AccountCellMapItem { val := ID_CELL } {
+    acctID := { val := ID_CELL },
+    balance := _Gen25,
+    code := _Gen26,
+    storage := { val := STORAGE_CELL },
+    origStorage := _Gen27,
+    transientStorage := _Gen28,
+    nonce := _Gen29 } = some _Val8)
+  (defn_Val9 : _AccountCellMap_ _Val8 _DotVar6 = some _Val9)
+  (defn_Val10 : lookup STORAGE_CELL W0 = some _Val10)
+  (defn_Val11 : «_+Int_» PC_CELL 1 = some _Val11)
+  (defn_Val12 : «#inStorage» ACCESSEDSTORAGE_CELL ((@inj SortInt SortAccount) ID_CELL) W0 = some _Val12)
+  (defn_Val13 : «_<_>_SCHEDULE_Int_ScheduleConst_Schedule» SortScheduleConst.Gwarmstorageread_SCHEDULE_ScheduleConst SCHEDULE_CELL = some _Val13)
+  (defn_Val14 : «_<_>_SCHEDULE_Int_ScheduleConst_Schedule» SortScheduleConst.Gcoldsload_SCHEDULE_ScheduleConst SCHEDULE_CELL = some _Val14)
+  (defn_Val15 : kite _Val12 _Val13 _Val14 = some _Val15)
+  (defn_Val16 : «_-Int_» GAS_CELL _Val15 = some _Val16)
+  (defn_Val17 : «.Set» = some _Val17)
+  (defn_Val18 : «Map:lookupOrDefault» ACCESSEDSTORAGE_CELL ((@inj SortInt SortKItem) ID_CELL) ((@inj SortSet SortKItem) _Val17) = some _Val18)
+  (defn_Val19 : «project:Set» (SortK.kseq _Val18 SortK.dotk) = some _Val19)
+  (defn_Val20 : SetItem ((@inj SortInt SortKItem) W0) = some _Val20)
+  (defn_Val21 : «_|Set__SET_Set_Set_Set» _Val19 _Val20 = some _Val21)
+  (defn_Val22 : «Map:update» ACCESSEDSTORAGE_CELL ((@inj SortInt SortKItem) ID_CELL) ((@inj SortSet SortKItem) _Val21) = some _Val22)
+  (defn_Val23 : AccountCellMapItem { val := ID_CELL } {
+    acctID := { val := ID_CELL },
+    balance := _Gen25,
+    code := _Gen26,
+    storage := { val := STORAGE_CELL },
+    origStorage := _Gen27,
+    transientStorage := _Gen28,
+    nonce := _Gen29 } = some _Val23)
+  (defn_Val24 : _AccountCellMap_ _Val23 _DotVar6 = some _Val24)
+  (req : _Val7 = true) :
+  Rewrites
+  (@sloadLHS ACCESSEDSTORAGE_CELL GAS_CELL ID_CELL PC_CELL W0 K_CELL SCHEDULE_CELL USEGAS_CELL WS _DotVar0 _DotVar6 _Val9 _Gen0 _Gen1 _Gen10 _Gen11 _Gen12 _Gen13 _Gen14 _Gen15 _Gen16 _Gen17 _Gen18 _Gen19 _Gen2 _Gen20 _Gen21 _Gen22 _Gen23 _Gen24 _Gen25 _Gen26 _Gen27 _Gen28 _Gen29 _Gen3 _Gen30 _Gen31 _Gen32 _Gen33 _Gen34 _Gen35 _Gen36 _Gen37 _Gen38 _Gen4 _Gen5 _Gen6 _Gen7 _Gen8 _Gen9)
+  (@sloadRHS _Val22 ID_CELL _Val10 _Val11 _Val13 _Val14 _Val15 _Val16 _Val2 _Val3 _Val4 K_CELL SCHEDULE_CELL _Val0 _Val1 _Val12 _Val5 _Val6 _Val7 WS _DotVar0 _DotVar6 _Val23 _Val24 _Val8 _Val9 _Gen0 _Gen1 _Gen10 _Gen11 _Gen12 _Gen13 _Gen14 _Gen15 _Gen16 _Gen17 _Gen18 _Gen19 _Gen2 _Gen20 _Gen21 _Gen22 _Gen23 _Gen24 _Gen25 _Gen26 _Gen27 _Gen28 _Gen29 _Gen3 _Gen30 _Gen31 _Gen32 _Gen33 _Gen34 _Gen35 _Gen36 _Gen37 _Gen38 _Gen4 _Gen5 _Gen6 _Gen7 _Gen8 _Gen9 _Val17 _Val19 _Val20 _Val21 _Val18) := by
+  apply (@Rewrites.SLOAD_SUMMARY_SLOAD_SUMMARY_1 ACCESSEDSTORAGE_CELL STORAGE_CELL _Val22 GAS_CELL ID_CELL PC_CELL W0 _Val10 _Val11 _Val13 _Val14 _Val15 _Val16 _Val2 _Val3 _Val4 K_CELL SCHEDULE_CELL USEGAS_CELL _Val0 _Val1 _Val12 _Val5 _Val6 _Val7 WS _DotVar0 _DotVar6 _Val23 _Val24 _Val8 _Val9 _Gen0 _Gen1 _Gen10 _Gen11 _Gen12 _Gen13 _Gen14 _Gen15 _Gen16 _Gen17 _Gen18 _Gen19 _Gen2 _Gen20 _Gen21 _Gen22 _Gen23 _Gen24 _Gen25 _Gen26 _Gen27 _Gen28 _Gen29 _Gen3 _Gen30 _Gen31 _Gen32 _Gen33 _Gen34 _Gen35 _Gen36 _Gen37 _Gen38 _Gen4 _Gen5 _Gen6 _Gen7 _Gen8 _Gen9 _Val17 _Val19 _Val20 _Val21 _Val18)
+  all_goals assumption
+
+theorem sload_prestate_equiv
+  {ACCESSEDSTORAGE_CELL : SortMap}
+  {GAS_CELL ID_CELL PC_CELL W0 : SortInt}
+  {K_CELL : SortK}
+  {SCHEDULE_CELL : SortSchedule}
+  {USEGAS_CELL : SortBool}
+  {WS : SortWordStack}
+  {_DotVar0 : SortGeneratedCounterCell}
+  {_DotVar6 _Val9 : SortAccountCellMap}
+  {_Gen0 : SortProgramCell}
+  {_Gen1 : SortJumpDestsCell}
+  {_Gen10 : SortSelfDestructCell}
+  {_Gen11 : SortLogCell}
+  {_Gen12 : SortRefundCell}
+  {_Gen13 : SortAccessedAccountsCell}
+  {_Gen14 : SortCreatedAccountsCell}
+  {_Gen15 : SortOutputCell}
+  {_Gen16 : SortStatusCodeCell}
+  {_Gen17 : SortCallStackCell}
+  {_Gen18 : SortInterimStatesCell}
+  {_Gen19 : SortTouchedAccountsCell}
+  {_Gen2 : SortCallerCell}
+  {_Gen20 : SortVersionedHashesCell}
+  {_Gen21 : SortGasPriceCell}
+  {_Gen22 : SortOriginCell}
+  {_Gen23 : SortBlockhashesCell}
+  {_Gen24 : SortBlockCell}
+  {_Gen25 : SortBalanceCell}
+  {_Gen26 : SortCodeCell}
+  {_Gen27 : SortOrigStorageCell}
+  {_Gen28 : SortTransientStorageCell}
+  {_Gen29 : SortNonceCell}
+  {_Gen3 : SortCallDataCell}
+  {_Gen30 : SortChainIDCell}
+  {_Gen31 : SortTxOrderCell}
+  {_Gen32 : SortTxPendingCell}
+  {_Gen33 : SortMessagesCell}
+  {_Gen34 : SortWithdrawalsPendingCell}
+  {_Gen35 : SortWithdrawalsOrderCell}
+  {_Gen36 : SortWithdrawalsCell}
+  {_Gen37 : SortExitCodeCell}
+  {_Gen38 : SortModeCell}
+  {_Gen4 : SortCallValueCell}
+  {_Gen5 : SortLocalMemCell}
+  {_Gen6 : SortMemoryUsedCell}
+  {_Gen7 : SortCallGasCell}
+  {_Gen8 : SortStaticCell}
+  {_Gen9 : SortCallDepthCell}
+  (symState : EVM.State):
+  let lhs := @sloadLHS ACCESSEDSTORAGE_CELL GAS_CELL ID_CELL PC_CELL W0 K_CELL SCHEDULE_CELL USEGAS_CELL WS _DotVar0 _DotVar6 _Val9 _Gen0 _Gen1 _Gen10 _Gen11 _Gen12 _Gen13 _Gen14 _Gen15 _Gen16 _Gen17 _Gen18 _Gen19 _Gen2 _Gen20 _Gen21 _Gen22 _Gen23 _Gen24 _Gen25 _Gen26 _Gen27 _Gen28 _Gen29 _Gen3 _Gen30 _Gen31 _Gen32 _Gen33 _Gen34 _Gen35 _Gen36 _Gen37 _Gen38 _Gen4 _Gen5 _Gen6 _Gen7 _Gen8 _Gen9
+  stateMap symState lhs =
+  {symState with
+    stack := (intMap W0) :: wordStackMap WS
+    pc := intMap PC_CELL
+    gasAvailable := intMap GAS_CELL
+    executionEnv := {symState.executionEnv with
+                  code := _Gen0.val,
+                  codeOwner := accountAddressMap ((@inj SortInt SortAccount) ID_CELL)
+                  perm := !lhs.isStatic.val},
+    substate := {symState.substate with
+            accessedStorageKeys :=  Axioms.SortAccessedStorageCellMap (SortGeneratedTopCell.accessedStorage lhs)
+            refundBalance := intMap lhs.refund.val
+           }
+    returnData := _Gen15.val
+    accountMap := Axioms.SortAccountsCellMap lhs.accounts
+    } := by rfl
+
+theorem sload_poststate_equiv
+  -- We have to include `ACCESSEDSTORAGE_CELL` as we need the original map to look up
+  {ACCESSEDSTORAGE_CELL _Val22 : SortMap}
+  -- We have to include `W0` as we need the key to look up
+  {GAS_CELL ID_CELL PC_CELL W0 _Val10 _Val11 _Val13 _Val14 _Val15 _Val16 _Val2 _Val3 _Val4 : SortInt}
+  {K_CELL : SortK}
+  {SCHEDULE_CELL : SortSchedule}
+  {_Val0 _Val1 _Val12 _Val5 _Val6 _Val7 : SortBool}
+  {WS : SortWordStack}
+  {_DotVar0 : SortGeneratedCounterCell}
+  {_DotVar6 _Val23 _Val24 _Val8 _Val9 : SortAccountCellMap}
+  {_Gen0 : SortProgramCell}
+  {_Gen1 : SortJumpDestsCell}
+  {_Gen10 : SortSelfDestructCell}
+  {_Gen11 : SortLogCell}
+  {_Gen12 : SortRefundCell}
+  {_Gen13 : SortAccessedAccountsCell}
+  {_Gen14 : SortCreatedAccountsCell}
+  {_Gen15 : SortOutputCell}
+  {_Gen16 : SortStatusCodeCell}
+  {_Gen17 : SortCallStackCell}
+  {_Gen18 : SortInterimStatesCell}
+  {_Gen19 : SortTouchedAccountsCell}
+  {_Gen2 : SortCallerCell}
+  {_Gen20 : SortVersionedHashesCell}
+  {_Gen21 : SortGasPriceCell}
+  {_Gen22 : SortOriginCell}
+  {_Gen23 : SortBlockhashesCell}
+  {_Gen24 : SortBlockCell}
+  {_Gen25 : SortBalanceCell}
+  {_Gen26 : SortCodeCell}
+  {_Gen27 : SortOrigStorageCell}
+  {_Gen28 : SortTransientStorageCell}
+  {_Gen29 : SortNonceCell}
+  {_Gen3 : SortCallDataCell}
+  {_Gen30 : SortChainIDCell}
+  {_Gen31 : SortTxOrderCell}
+  {_Gen32 : SortTxPendingCell}
+  {_Gen33 : SortMessagesCell}
+  {_Gen34 : SortWithdrawalsPendingCell}
+  {_Gen35 : SortWithdrawalsOrderCell}
+  {_Gen36 : SortWithdrawalsCell}
+  {_Gen37 : SortExitCodeCell}
+  {_Gen38 : SortModeCell}
+  {_Gen4 : SortCallValueCell}
+  {_Gen5 : SortLocalMemCell}
+  {_Gen6 : SortMemoryUsedCell}
+  {_Gen7 : SortCallGasCell}
+  {_Gen8 : SortStaticCell}
+  {_Gen9 : SortCallDepthCell}
+  {_Val17 _Val19 _Val20 _Val21 : SortSet}
+  {_Val18 : SortKItem}
+  (defn_Val11 : «_+Int_» PC_CELL 1 = some _Val11)
+  (defn_Val12 : «#inStorage» ACCESSEDSTORAGE_CELL ((@inj SortInt SortAccount) ID_CELL) W0 = some _Val12)
+  (defn_Val13 : «_<_>_SCHEDULE_Int_ScheduleConst_Schedule» SortScheduleConst.Gwarmstorageread_SCHEDULE_ScheduleConst SCHEDULE_CELL = some _Val13)
+  (defn_Val14 : «_<_>_SCHEDULE_Int_ScheduleConst_Schedule» SortScheduleConst.Gcoldsload_SCHEDULE_ScheduleConst SCHEDULE_CELL = some _Val14)
+  (defn_Val15 : kite _Val12 _Val13 _Val14 = some _Val15)
+  (defn_Val16 : «_-Int_» GAS_CELL _Val15 = some _Val16)
+  (gasEnough : _Val15 ≤ GAS_CELL)
+  (gasSmall : GAS_CELL < ↑UInt256.size)
+  (cancun : SCHEDULE_CELL = .CANCUN_EVM)
+  (symState : EVM.State) :
+  let rhs := @sloadRHS _Val22 ID_CELL _Val10 _Val11 _Val13 _Val14 _Val15 _Val16 _Val2 _Val3 _Val4 K_CELL SCHEDULE_CELL _Val0 _Val1 _Val12 _Val5 _Val6 _Val7 WS _DotVar0 _DotVar6 _Val23 _Val24 _Val8 _Val9 _Gen0 _Gen1 _Gen10 _Gen11 _Gen12 _Gen13 _Gen14 _Gen15 _Gen16 _Gen17 _Gen18 _Gen19 _Gen2 _Gen20 _Gen21 _Gen22 _Gen23 _Gen24 _Gen25 _Gen26 _Gen27 _Gen28 _Gen29 _Gen3 _Gen30 _Gen31 _Gen32 _Gen33 _Gen34 _Gen35 _Gen36 _Gen37 _Gen38 _Gen4 _Gen5 _Gen6 _Gen7 _Gen8 _Gen9 _Val17 _Val19 _Val20 _Val21 _Val18
+  stateMap symState rhs =
+  {symState with
+    stack := intMap _Val10 :: wordStackMap WS
+    pc := intMap («_+Int'_» PC_CELL 1)
+    gasAvailable := intMap GAS_CELL -  intMap _Val15 --(sload_gas ACCESSEDSTORAGE_CELL W0)
+    executionEnv := {symState.executionEnv with
+                  code := _Gen0.val,
+                  codeOwner := accountAddressMap ((@inj SortInt SortAccount) ID_CELL)
+                  perm := !rhs.isStatic.val},
+    accountMap := Axioms.SortAccountsCellMap rhs.accounts
+    substate := {symState.substate with
+            accessedStorageKeys :=  Axioms.SortAccessedStorageCellMap  rhs.accessedStorage
+            refundBalance := intMap _Gen12.val
+           }
+    returnData := _Gen15.val
+  } := by
+  simp_all [sloadRHS, stateMap, «_-Int_», plusInt_def, «_+Int_»]
+  aesop (add simp [inj, Inj.inj]) (add safe (by rw [intMap_sub_dist]))
+
+theorem step_sload_equiv
+  {ACCESSEDSTORAGE_CELL STORAGE_CELL _Val22 : SortMap}
+  {GAS_CELL ID_CELL PC_CELL W0 _Val10 _Val11 _Val13 _Val14 _Val15 _Val16 _Val2 _Val3 _Val4 : SortInt}
+  {K_CELL : SortK}
+  {SCHEDULE_CELL : SortSchedule}
+  {USEGAS_CELL _Val0 _Val1 _Val12 _Val5 _Val6 _Val7 : SortBool}
+  {WS : SortWordStack}
+  {_DotVar0 : SortGeneratedCounterCell}
+  {_DotVar6 _Val23 _Val24 _Val8 _Val9 : SortAccountCellMap}
+  {_Gen0 : SortProgramCell}
+  {_Gen1 : SortJumpDestsCell}
+  {_Gen10 : SortSelfDestructCell}
+  {_Gen11 : SortLogCell}
+  {_Gen12 : SortRefundCell}
+  {_Gen13 : SortAccessedAccountsCell}
+  {_Gen14 : SortCreatedAccountsCell}
+  {_Gen15 : SortOutputCell}
+  {_Gen16 : SortStatusCodeCell}
+  {_Gen17 : SortCallStackCell}
+  {_Gen18 : SortInterimStatesCell}
+  {_Gen19 : SortTouchedAccountsCell}
+  {_Gen2 : SortCallerCell}
+  {_Gen20 : SortVersionedHashesCell}
+  {_Gen21 : SortGasPriceCell}
+  {_Gen22 : SortOriginCell}
+  {_Gen23 : SortBlockhashesCell}
+  {_Gen24 : SortBlockCell}
+  {_Gen25 : SortBalanceCell}
+  {_Gen26 : SortCodeCell}
+  {_Gen27 : SortOrigStorageCell}
+  {_Gen28 : SortTransientStorageCell}
+  {_Gen29 : SortNonceCell}
+  {_Gen3 : SortCallDataCell}
+  {_Gen30 : SortChainIDCell}
+  {_Gen31 : SortTxOrderCell}
+  {_Gen32 : SortTxPendingCell}
+  {_Gen33 : SortMessagesCell}
+  {_Gen34 : SortWithdrawalsPendingCell}
+  {_Gen35 : SortWithdrawalsOrderCell}
+  {_Gen36 : SortWithdrawalsCell}
+  {_Gen37 : SortExitCodeCell}
+  {_Gen38 : SortModeCell}
+  {_Gen4 : SortCallValueCell}
+  {_Gen5 : SortLocalMemCell}
+  {_Gen6 : SortMemoryUsedCell}
+  {_Gen7 : SortCallGasCell}
+  {_Gen8 : SortStaticCell}
+  {_Gen9 : SortCallDepthCell}
+  {_Val17 _Val19 _Val20 _Val21 : SortSet}
+  {_Val18 : SortKItem}
+  (defn_Val0 : «_<<_>>_SCHEDULE_Bool_ScheduleFlag_Schedule» SortScheduleFlag.Ghasaccesslist_SCHEDULE_ScheduleFlag SCHEDULE_CELL = some _Val0)
+  (defn_Val1 : «#inStorage» ACCESSEDSTORAGE_CELL ((@inj SortInt SortAccount) ID_CELL) W0 = some _Val1)
+  (defn_Val2 : «_<_>_SCHEDULE_Int_ScheduleConst_Schedule» SortScheduleConst.Gwarmstorageread_SCHEDULE_ScheduleConst SCHEDULE_CELL = some _Val2)
+  (defn_Val3 : «_<_>_SCHEDULE_Int_ScheduleConst_Schedule» SortScheduleConst.Gcoldsload_SCHEDULE_ScheduleConst SCHEDULE_CELL = some _Val3)
+  (defn_Val4 : kite _Val1 _Val2 _Val3 = some _Val4)
+  (defn_Val5 : «_<=Int_» _Val4 GAS_CELL = some _Val5)
+  /- (defn_Val6 : _andBool_ _Val0 _Val5 = some _Val6) -/
+  (defn_Val7 : _andBool_ USEGAS_CELL _Val6 = some _Val7)
+  (defn_Val8 : AccountCellMapItem { val := ID_CELL } {
+    acctID := { val := ID_CELL },
+    balance := _Gen25,
+    code := _Gen26,
+    storage := { val := STORAGE_CELL },
+    origStorage := _Gen27,
+    transientStorage := _Gen28,
+    nonce := _Gen29 } = some _Val8)
+  (defn_Val9 : _AccountCellMap_ _Val8 _DotVar6 = some _Val9)
+  (defn_Val10 : lookup STORAGE_CELL W0 = some _Val10)
+  (defn_Val11 : «_+Int_» PC_CELL 1 = some _Val11)
+  (defn_Val12 : «#inStorage» ACCESSEDSTORAGE_CELL ((@inj SortInt SortAccount) ID_CELL) W0 = some _Val12)
+  (defn_Val13 : «_<_>_SCHEDULE_Int_ScheduleConst_Schedule» SortScheduleConst.Gwarmstorageread_SCHEDULE_ScheduleConst SCHEDULE_CELL = some _Val13)
+  (defn_Val14 : «_<_>_SCHEDULE_Int_ScheduleConst_Schedule» SortScheduleConst.Gcoldsload_SCHEDULE_ScheduleConst SCHEDULE_CELL = some _Val14)
+  (defn_Val15 : kite _Val12 _Val13 _Val14 = some _Val15)
+  (defn_Val16 : «_-Int_» GAS_CELL _Val15 = some _Val16)
+  (defn_Val17 : «.Set» = some _Val17)
+  (defn_Val18 : «Map:lookupOrDefault» ACCESSEDSTORAGE_CELL ((@inj SortInt SortKItem) ID_CELL) ((@inj SortSet SortKItem) _Val17) = some _Val18)
+  (defn_Val19 : «project:Set» (SortK.kseq _Val18 SortK.dotk) = some _Val19)
+  (defn_Val20 : SetItem ((@inj SortInt SortKItem) W0) = some _Val20)
+  (defn_Val21 : «_|Set__SET_Set_Set_Set» _Val19 _Val20 = some _Val21)
+  (defn_Val22 : «Map:update» ACCESSEDSTORAGE_CELL ((@inj SortInt SortKItem) ID_CELL) ((@inj SortSet SortKItem) _Val21) = some _Val22)
+  (defn_Val23 : AccountCellMapItem { val := ID_CELL } {
+    acctID := { val := ID_CELL },
+    balance := _Gen25,
+    code := _Gen26,
+    storage := { val := STORAGE_CELL },
+    origStorage := _Gen27,
+    transientStorage := _Gen28,
+    nonce := _Gen29 } = some _Val23)
+  (defn_Val24 : _AccountCellMap_ _Val23 _DotVar6 = some _Val24)
+  (req : _Val7 = true)
+  (symState : EVM.State)
+  -- needed for EVM.step
+  (gasCost : ℕ)
+  -- Necessary assumptions for equivalence
+  (cancun : SCHEDULE_CELL = .CANCUN_EVM)
+  (gavailEnough : _Val15 ≤ GAS_CELL)
+  (gavailSmall : GAS_CELL < ↑UInt256.size)
+  (gasCostValue : gasCost = _Val15.toNat)
+  (pcountSmall : PC_CELL + 1 < UInt256.size)
+  (pcountNonneg : 0 ≤ PC_CELL):
+  EVM.step_sload (Int.toNat GAS_CELL) gasCost (stateMap symState (@sloadLHS ACCESSEDSTORAGE_CELL GAS_CELL ID_CELL PC_CELL W0 K_CELL SCHEDULE_CELL USEGAS_CELL WS _DotVar0 _DotVar6 _Val9 _Gen0 _Gen1 _Gen10 _Gen11 _Gen12 _Gen13 _Gen14 _Gen15 _Gen16 _Gen17 _Gen18 _Gen19 _Gen2 _Gen20 _Gen21 _Gen22 _Gen23 _Gen24 _Gen25 _Gen26 _Gen27 _Gen28 _Gen29 _Gen3 _Gen30 _Gen31 _Gen32 _Gen33 _Gen34 _Gen35 _Gen36 _Gen37 _Gen38 _Gen4 _Gen5 _Gen6 _Gen7 _Gen8 _Gen9)) =
+  .ok (stateMap {symState with execLength := symState.execLength + 1} (@sloadRHS _Val22 ID_CELL _Val10 _Val11 _Val13 _Val14 _Val15 _Val16 _Val2 _Val3 _Val4 K_CELL SCHEDULE_CELL _Val0 _Val1 _Val12 _Val5 _Val6 _Val7 WS _DotVar0 _DotVar6 _Val23 _Val24 _Val8 _Val9 _Gen0 _Gen1 _Gen10 _Gen11 _Gen12 _Gen13 _Gen14 _Gen15 _Gen16 _Gen17 _Gen18 _Gen19 _Gen2 _Gen20 _Gen21 _Gen22 _Gen23 _Gen24 _Gen25 _Gen26 _Gen27 _Gen28 _Gen29 _Gen3 _Gen30 _Gen31 _Gen32 _Gen33 _Gen34 _Gen35 _Gen36 _Gen37 _Gen38 _Gen4 _Gen5 _Gen6 _Gen7 _Gen8 _Gen9 _Val17 _Val19 _Val20 _Val21 _Val18)) := by
+  cases cg: (Int.toNat GAS_CELL)
+  next =>
+    have val15_pos : 0 < _Val15 := by simp at defn_Val15; aesop
+    have _ := Int.lt_of_lt_of_le val15_pos gavailEnough
+    omega
+  rw [sload_prestate_equiv, EVM.step_sload_summary] <;> try assumption
+  rw [sloadLHS, sload_poststate_equiv, sloadRHS] <;> try congr
+  . simp[State.lookupAccount, SortGeneratedTopCell.accounts, accountAddressMap, inj_ID_CELL]
+    aesop
+  . simp
+    apply (Axioms.accessedStorageCell_map_insert defn_Val17 defn_Val18 defn_Val19 defn_Val20 defn_Val21 defn_Val22)
+  . simp at defn_Val4; aesop (add simp [intMap])
+  . rw [plusInt_def, ←UInt256.add_succ_mod_size, intMap_add_dist] <;> aesop
+  . simp [State.lookupAccount]
+    cases origc: _Gen27; next orig_storage =>
+    rw [@Axioms.findAccountInAccountCellMap ID_CELL _Gen25 _Gen26 STORAGE_CELL orig_storage _Gen28 _Gen29 _Val8 _DotVar6 _Val9]
+     <;> congr
+    . simp [Account.lookupStorage]; apply Axioms.lookup_mapped_storage; assumption
+    . rw [←origc]; assumption
+  . omega
+
+theorem X_sload_equiv
+  {ACCESSEDSTORAGE_CELL STORAGE_CELL _Val22 : SortMap}
+  {GAS_CELL ID_CELL PC_CELL W0 _Val10 _Val11 _Val13 _Val14 _Val15 _Val16 _Val2 _Val3 _Val4 : SortInt}
+  {K_CELL : SortK}
+  {SCHEDULE_CELL : SortSchedule}
+  {USEGAS_CELL _Val0 _Val1 _Val12 _Val5 _Val6 _Val7 : SortBool}
+  {WS : SortWordStack}
+  {_DotVar0 : SortGeneratedCounterCell}
+  {_DotVar6 _Val23 _Val24 _Val8 _Val9 : SortAccountCellMap}
+  {_Gen0 : SortProgramCell}
+  {_Gen1 : SortJumpDestsCell}
+  {_Gen10 : SortSelfDestructCell}
+  {_Gen11 : SortLogCell}
+  {_Gen12 : SortRefundCell}
+  {_Gen13 : SortAccessedAccountsCell}
+  {_Gen14 : SortCreatedAccountsCell}
+  {_Gen15 : SortOutputCell}
+  {_Gen16 : SortStatusCodeCell}
+  {_Gen17 : SortCallStackCell}
+  {_Gen18 : SortInterimStatesCell}
+  {_Gen19 : SortTouchedAccountsCell}
+  {_Gen2 : SortCallerCell}
+  {_Gen20 : SortVersionedHashesCell}
+  {_Gen21 : SortGasPriceCell}
+  {_Gen22 : SortOriginCell}
+  {_Gen23 : SortBlockhashesCell}
+  {_Gen24 : SortBlockCell}
+  {_Gen25 : SortBalanceCell}
+  {_Gen26 : SortCodeCell}
+  {_Gen27 : SortOrigStorageCell}
+  {_Gen28 : SortTransientStorageCell}
+  {_Gen29 : SortNonceCell}
+  {_Gen3 : SortCallDataCell}
+  {_Gen30 : SortChainIDCell}
+  {_Gen31 : SortTxOrderCell}
+  {_Gen32 : SortTxPendingCell}
+  {_Gen33 : SortMessagesCell}
+  {_Gen34 : SortWithdrawalsPendingCell}
+  {_Gen35 : SortWithdrawalsOrderCell}
+  {_Gen36 : SortWithdrawalsCell}
+  {_Gen37 : SortExitCodeCell}
+  {_Gen38 : SortModeCell}
+  {_Gen4 : SortCallValueCell}
+  {_Gen5 : SortLocalMemCell}
+  {_Gen6 : SortMemoryUsedCell}
+  {_Gen7 : SortCallGasCell}
+  {_Gen8 : SortStaticCell}
+  {_Gen9 : SortCallDepthCell}
+  {_Val17 _Val19 _Val20 _Val21 : SortSet}
+  {_Val18 : SortKItem}
+  (defn_Val0 : «_<<_>>_SCHEDULE_Bool_ScheduleFlag_Schedule» SortScheduleFlag.Ghasaccesslist_SCHEDULE_ScheduleFlag SCHEDULE_CELL = some _Val0)
+  (defn_Val1 : «#inStorage» ACCESSEDSTORAGE_CELL ((@inj SortInt SortAccount) ID_CELL) W0 = some _Val1)
+  (defn_Val2 : «_<_>_SCHEDULE_Int_ScheduleConst_Schedule» SortScheduleConst.Gwarmstorageread_SCHEDULE_ScheduleConst SCHEDULE_CELL = some _Val2)
+  (defn_Val3 : «_<_>_SCHEDULE_Int_ScheduleConst_Schedule» SortScheduleConst.Gcoldsload_SCHEDULE_ScheduleConst SCHEDULE_CELL = some _Val3)
+  (defn_Val4 : kite _Val1 _Val2 _Val3 = some _Val4)
+  (defn_Val5 : «_<=Int_» _Val4 GAS_CELL = some _Val5)
+  /- (defn_Val6 : _andBool_ _Val0 _Val5 = some _Val6) -/
+  (defn_Val7 : _andBool_ USEGAS_CELL _Val6 = some _Val7)
+  (defn_Val8 : AccountCellMapItem { val := ID_CELL } {
+    acctID := { val := ID_CELL },
+    balance := _Gen25,
+    code := _Gen26,
+    storage := { val := STORAGE_CELL },
+    origStorage := _Gen27,
+    transientStorage := _Gen28,
+    nonce := _Gen29 } = some _Val8)
+  (defn_Val9 : _AccountCellMap_ _Val8 _DotVar6 = some _Val9)
+  (defn_Val10 : lookup STORAGE_CELL W0 = some _Val10)
+  (defn_Val11 : «_+Int_» PC_CELL 1 = some _Val11)
+  (defn_Val12 : «#inStorage» ACCESSEDSTORAGE_CELL ((@inj SortInt SortAccount) ID_CELL) W0 = some _Val12)
+  (defn_Val13 : «_<_>_SCHEDULE_Int_ScheduleConst_Schedule» SortScheduleConst.Gwarmstorageread_SCHEDULE_ScheduleConst SCHEDULE_CELL = some _Val13)
+  (defn_Val14 : «_<_>_SCHEDULE_Int_ScheduleConst_Schedule» SortScheduleConst.Gcoldsload_SCHEDULE_ScheduleConst SCHEDULE_CELL = some _Val14)
+  (defn_Val15 : kite _Val12 _Val13 _Val14 = some _Val15)
+  (defn_Val16 : «_-Int_» GAS_CELL _Val15 = some _Val16)
+  (defn_Val17 : «.Set» = some _Val17)
+  (defn_Val18 : «Map:lookupOrDefault» ACCESSEDSTORAGE_CELL ((@inj SortInt SortKItem) ID_CELL) ((@inj SortSet SortKItem) _Val17) = some _Val18)
+  (defn_Val19 : «project:Set» (SortK.kseq _Val18 SortK.dotk) = some _Val19)
+  (defn_Val20 : SetItem ((@inj SortInt SortKItem) W0) = some _Val20)
+  (defn_Val21 : «_|Set__SET_Set_Set_Set» _Val19 _Val20 = some _Val21)
+  (defn_Val22 : «Map:update» ACCESSEDSTORAGE_CELL ((@inj SortInt SortKItem) ID_CELL) ((@inj SortSet SortKItem) _Val21) = some _Val22)
+  (defn_Val23 : AccountCellMapItem { val := ID_CELL } {
+    acctID := { val := ID_CELL },
+    balance := _Gen25,
+    code := _Gen26,
+    storage := { val := STORAGE_CELL },
+    origStorage := _Gen27,
+    transientStorage := _Gen28,
+    nonce := _Gen29 } = some _Val23)
+  (defn_Val24 : _AccountCellMap_ _Val23 _DotVar6 = some _Val24)
+  (req : _Val7 = true)
+  (symState : EVM.State)
+  -- Necessary assumptions for equivalence
+  (cancun : SCHEDULE_CELL = .CANCUN_EVM)
+  (gavailEnough : _Val15 < GAS_CELL)
+  (gavailSmall : GAS_CELL < ↑UInt256.size)
+  (codeSloadLHS : _Gen0 = ⟨⟨#[(0x54 : UInt8)]⟩⟩)
+  (codeSloadRHS : _Gen26 = ⟨⟨⟨#[(0x54 : UInt8)]⟩⟩⟩)
+  (pcZero : PC_CELL = 0)
+  (wordStackOk : sizeWordStackAux WS 0 < some 1024)
+  :
+  EVM.X false (UInt256.toNat (intMap GAS_CELL)) (stateMap symState (@sloadLHS ACCESSEDSTORAGE_CELL GAS_CELL ID_CELL PC_CELL W0 K_CELL SCHEDULE_CELL USEGAS_CELL WS _DotVar0 _DotVar6 _Val9 _Gen0 _Gen1 _Gen10 _Gen11 _Gen12 _Gen13 _Gen14 _Gen15 _Gen16 _Gen17 _Gen18 _Gen19 _Gen2 _Gen20 _Gen21 _Gen22 _Gen23 _Gen24 _Gen25 _Gen26 _Gen27 _Gen28 _Gen29 _Gen3 _Gen30 _Gen31 _Gen32 _Gen33 _Gen34 _Gen35 _Gen36 _Gen37 _Gen38 _Gen4 _Gen5 _Gen6 _Gen7 _Gen8 _Gen9)) =
+  .ok (.success (stateMap {symState with execLength := symState.execLength + 2} (@sloadRHS _Val22 ID_CELL _Val10 _Val11 _Val13 _Val14 _Val15 _Val16 _Val2 _Val3 _Val4 K_CELL SCHEDULE_CELL _Val0 _Val1 _Val12 _Val5 _Val6 _Val7 WS _DotVar0 _DotVar6 _Val23 _Val24 _Val8 _Val9 _Gen0 _Gen1 _Gen10 _Gen11 _Gen12 _Gen13 _Gen14 ⟨.empty⟩ _Gen16 _Gen17 _Gen18 _Gen19 _Gen2 _Gen20 _Gen21 _Gen22 _Gen23 _Gen24 _Gen25 _Gen26 _Gen27 _Gen28 _Gen29 _Gen3 _Gen30 _Gen31 _Gen32 _Gen33 _Gen34 _Gen35 _Gen36 _Gen37 _Gen38 _Gen4 _Gen5 _Gen6 _Gen7 _Gen8 _Gen9 _Val17 _Val19 _Val20 _Val21 _Val18)) .empty ) := by
+  rw [pcZero, codeSloadLHS, codeSloadRHS, sload_prestate_equiv, sload_poststate_equiv]
+  <;> first | assumption | try linarith
+  simp
+  have pc_equiv : intMap 0 = UInt256.ofNat 0 := rfl
+  rw [pc_equiv, X_sload_summary] <;> try simp [State.lookupAccount, sloadLHS, sloadRHS]
+  <;> try assumption
+  . constructor <;> constructor
+    . rw [Axioms.accessedStorageCell_map_insert defn_Val17 defn_Val18 defn_Val19 defn_Val20 defn_Val21 defn_Val22]
+      aesop
+    . simp [EVM.Csload, GasConstants.Gwarmaccess, GasConstants.Gcoldsload]
+      simp [*] at defn_Val12 defn_Val13 defn_Val14 defn_Val15; congr
+      simp [←defn_Val13, ←defn_Val14, ←defn_Val15]
+      rw [Axioms.contains_accessedStorage_map defn_Val12]
+      aesop
+    . aesop
+    . cases origc: _Gen27; next orig_storage =>
+      rw [@Axioms.findAccountInAccountCellMap ID_CELL _Gen25 _Gen26 STORAGE_CELL orig_storage _Gen28 _Gen29 _Val8 _DotVar6 _Val9]
+      <;> congr
+      . simp [Account.lookupStorage]; apply Axioms.lookup_mapped_storage; assumption
+      . rw [←origc]; assumption
+  . simp_all [sizeWordStack_def]
+    simp [LT.lt, Option.lt, OfNat.ofNat, (@Int.ofNat_eq_coe 1024)] at wordStackOk
+    exact (Int.lt_of_ofNat_lt_ofNat wordStackOk)
+  . simp [EVM.Csload, GasConstants.Gwarmaccess, GasConstants.Gcoldsload]
+    rw [Axioms.contains_accessedStorage_map defn_Val12]
+    simp [cancun] at *; rw [intMap_toNat] <;> aesop (add safe (by linarith))
+
+end SloadOpcodeEquivalence
