EvmEquivalence/Summaries/SloadSummary.lean
@@ -1,0 +1,195 @@
+import EvmYul.EVM.Semantics
+import EvmYul.EVM.GasConstants
+import EvmEquivalence.Interfaces.EvmYulInterface
+
+open EvmYul
+open EVM
+open EvmYul.State
+
+namespace SloadSummary
+
+section
+
+variable (gas gasCost : ℕ)
+variable (symStack : Stack UInt256)
+variable (symPc symGasAvailable symRefund key value : UInt256)
+variable (symExecLength : ℕ)
+variable (symReturnData symCode : ByteArray)
+variable (symAccessedStorageKeys : Batteries.RBSet (AccountAddress × UInt256) Substate.storageKeysCmp)
+variable (symAccounts : AccountMap)
+variable (symCodeOwner : AccountAddress)
+variable (symPerm : Bool)
+
+@[simp]
+abbrev sloadEVM := @Operation.SLOAD .EVM
+
+@[simp]
+abbrev sload_instr : Option (Operation .EVM × Option (UInt256 × Nat)) :=
+  some ⟨sloadEVM, none⟩
+
+@[simp]
+abbrev EVM.step_sload : Transformer :=
+  EVM.step false gas gasCost sload_instr
+
+@[simp]
+abbrev EvmYul.step_sload : Transformer :=
+  EvmYul.step false sloadEVM
+
+@[simp]
+def lookupStorage_sload (symState : EvmYul.State) (key : UInt256) : UInt256 :=
+  let Iₐ := symState.executionEnv.codeOwner
+  match symState.lookupAccount Iₐ with
+  | none => ⟨0⟩
+  | some acc => acc.lookupStorage key
+
+theorem sload_summary (symState : EvmYul.State) (key : UInt256):
+  let ss := {symState with
+             executionEnv := {symState.executionEnv with
+                  code := symCode,
+                  codeOwner := symCodeOwner
+                  perm := symPerm},
+             substate := {symState.substate with
+                          accessedStorageKeys :=  symAccessedStorageKeys
+                          refundBalance := symRefund}
+             accountMap := symAccounts}
+  State.sload ss key =
+  (addAccessedStorageKey ss (symCodeOwner, key),
+    lookupStorage_sload ss key) := by
+  cases cco: (symState.lookupAccount symState.executionEnv.codeOwner)
+  all_goals aesop (add simp [sload, Option.option, lookupAccount, Substate.addAccessedStorageKey])
+
+/--
+Theorem needed to bypass the `private` attribute of `EVM.dispatchBinaryStateOp`
+ -/
+theorem sload_bypass_private (symState : EVM.State):
+  let ss := {symState with
+  stack := symStack,
+  pc := symPc
+  gasAvailable := symGasAvailable,
+  executionEnv := {symState.executionEnv with
+                  code := symCode,
+                  codeOwner := symCodeOwner
+                  perm := symPerm},
+  substate := {symState.substate with
+               accessedStorageKeys :=  symAccessedStorageKeys
+               refundBalance := symRefund}
+  returnData := symReturnData,
+  execLength := symExecLength,
+  accountMap := symAccounts}
+  EvmYul.step_sload ss =
+  EVM.unaryStateOp false EvmYul.State.sload ss := rfl
+
+theorem EvmYul.step_sload_summary (symState : EVM.State):
+  let ss := {symState with
+    stack := key :: symStack,
+    pc := symPc
+    gasAvailable := symGasAvailable,
+    executionEnv := {symState.executionEnv with
+                  code := symCode,
+                  codeOwner := symCodeOwner
+                  perm := symPerm},
+    substate := {symState.substate with
+                 accessedStorageKeys :=  symAccessedStorageKeys
+                 refundBalance := symRefund}
+    returnData := symReturnData,
+    execLength := symExecLength,
+    accountMap := symAccounts}
+  EvmYul.step_sload ss =
+  .ok {ss with
+    stack := lookupStorage_sload ss.toState key :: symStack,
+    pc := symPc + .ofNat 1
+    substate.accessedStorageKeys := ss.substate.accessedStorageKeys.insert ⟨ss.executionEnv.codeOwner, key⟩} := by
+  simp [sload_bypass_private, unaryStateOp, Stack.pop, Id.run, State.replaceStackAndIncrPC, State.incrPC, sload, lookupAccount]
+  aesop (add simp [sload_summary, Substate.addAccessedStorageKey])
+
+theorem EVM.step_sload_summary (gas_pos : 0 < gas) (symState : EVM.State):
+  let ss := {symState with
+    stack := key :: symStack,
+    pc := symPc
+    gasAvailable := symGasAvailable,
+    executionEnv := {symState.executionEnv with
+                  code := symCode,
+                  codeOwner := symCodeOwner
+                  perm := symPerm},
+    substate := {symState.substate with
+                 accessedStorageKeys :=  symAccessedStorageKeys
+                 refundBalance := symRefund}
+    returnData := symReturnData,
+    execLength := symExecLength,
+    accountMap := symAccounts}
+  EVM.step_sload gas gasCost ss =
+    .ok {ss with
+          stack := lookupStorage_sload ss.toState key :: symStack,
+          pc := symPc + (.ofNat 1),
+          gasAvailable := symGasAvailable - UInt256.ofNat gasCost,
+          substate := {ss.substate with
+            accessedStorageKeys := ss.substate.accessedStorageKeys.insert ⟨ss.executionEnv.codeOwner, key⟩
+           }
+          execLength := symExecLength + 1} := by
+  cases gas; contradiction
+  simp [step_sload, EVM.step]
+  have srw := EvmYul.step_sload_summary symStack symPc (symGasAvailable - UInt256.ofNat gasCost) symRefund key (symExecLength + 1) symReturnData symCode symAccessedStorageKeys symAccounts symCodeOwner symPerm
+  simp [EvmYul.step_sload, Operation.SLOAD] at srw; simp [srw]
+
+@[simp]
+theorem decode_singleton_sload :
+  decode ⟨#[0x54]⟩ (.ofNat 0) = some ⟨sloadEVM, none⟩ := rfl
+
+@[simp]
+theorem memoryExpansionCost_sload (symState : EVM.State) :
+  memoryExpansionCost symState sloadEVM = 0 := by
+  simp [memoryExpansionCost, memoryExpansionCost.μᵢ']
+
+/--
+TODO: Generalize to `C'`
+ -/
+theorem Csload_pos (symState : EVM.State) : 99 < Csload symState.stack symState.substate symState.executionEnv := by
+  aesop (add simp [Csload, GasConstants.Gcoldsload, GasConstants.Gwarmaccess])
+
+theorem X_sload_summary (symState : EVM.State)
+                         (symStack_ok : symStack.length < 1024):
+  let ss := {symState with
+    stack := key :: symStack,
+    pc := .ofNat 0
+    gasAvailable := symGasAvailable,
+    executionEnv := {symState.executionEnv with
+                  code := ⟨#[(0x54 : UInt8)]⟩,
+                  codeOwner := symCodeOwner
+                  perm := symPerm},
+    substate := {symState.substate with
+                 accessedStorageKeys :=  symAccessedStorageKeys
+                 refundBalance := symRefund}
+    returnData := symReturnData,
+    execLength := symExecLength,
+    accountMap := symAccounts}
+  Csload ss.stack ss.substate ss.executionEnv < symGasAvailable.toNat →
+  X false symGasAvailable.toNat ss =
+  .ok (.success {ss with
+          stack := lookupStorage_sload ss.toState key :: symStack,
+          pc := .ofNat 1,
+          gasAvailable := symGasAvailable - (.ofNat (Csload ss.stack ss.substate ss.executionEnv)),
+          substate := {ss.substate with
+            accessedStorageKeys := ss.substate.accessedStorageKeys.insert ⟨ss.executionEnv.codeOwner, key⟩
+           }
+          returnData := .empty,
+          execLength := symExecLength + 2} .empty) := by
+  intro ss enoughGas
+  have gavail_pos := Nat.lt_trans (Csload_pos ss) enoughGas
+  cases g_case : symGasAvailable.toNat; rw [g_case] at gavail_pos; contradiction
+  case succ g_pos =>
+  simp [X, C', δ]
+  have lt_fls_rw {n m : ℕ} (_ : n < m) : (m < n) = False := by
+    simp; apply Nat.ge_of_not_lt; simp; omega
+  simp [ss, (lt_fls_rw enoughGas), α, (lt_fls_rw symStack_ok)]
+  have stack_ok_rw : (1024 < List.length symStack + 1) = False := by
+    aesop (add safe (by linarith))
+  simp [stack_ok_rw]; split; contradiction; next evm cost stateOk =>
+  have step_rw := (EVM.step_sload_summary g_pos (Csload ss.stack ss.substate ss.executionEnv) symStack (.ofNat 0)
+    symGasAvailable symRefund key symExecLength symReturnData ⟨#[(0x54 : UInt8)]⟩
+    symAccessedStorageKeys symAccounts symCodeOwner symPerm (by omega) evm)
+  cases stateOk; simp at step_rw; rw [step_rw]; simp [Except.instMonad, Except.bind]
+  rw [X_bad_pc] <;> aesop (add safe (by omega))
+
+end
+
+end SloadSummary
